src/bico/working examples/java_lang_Object.v
@@ -1,0 +1,44 @@
+  Module java_lang_Object.
+
+    Definition className : ClassName := (javaLang, object). 
+
+    Definition _init_Signature : MethodSignature := METHODSIGNATURE.Build_t
+      (className, 10%positive)
+      nil
+      None
+    .
+
+    Definition _init_Instructions : list (PC*Instruction) :=
+      (0%N, Return)::
+      nil
+    .
+
+    Definition _init_Body : BytecodeMethod := BYTECODEMETHOD.Build_t
+      _init_Instructions
+      nil
+      1
+      0
+    .
+
+    Definition _init_Method : Method := METHOD.Build_t
+      _init_Signature
+      (Some _init_Body)
+      false
+      false
+      false
+      Public
+    .
+
+    Definition class : Class := CLASS.Build_t
+      className
+      None (* (Some java_lang_Object.className) *)
+      nil
+      nil
+      (_init_Method::nil)
+      false
+      true
+      false
+    .
+
+  End java_lang_Object.
+    
