src/bico/working examples/java_lang_Throwable.v
@@ -1,0 +1,51 @@
+  Module java_lang_Throwable.
+
+    Definition className : ClassName := (javaLang, throwable). 
+
+    Definition _init_Signature : MethodSignature := METHODSIGNATURE.Build_t
+      (className, 10%positive)
+      nil
+      None
+    .
+
+    Definition _init_Instructions : list (PC*Instruction) :=
+      (0%N, Vload Aval 0%N)::
+      (1%N, Invokespecial java_lang_Object._init_Signature)::
+      (4%N, Vload Aval 0%N)::
+      (5%N, Vload Aval 0%N)::
+      (6%N, Putfield java_lang_Throwable.causeFieldSignature)::
+      (9%N, Vload Aval 0%N)::
+      (10%N, Invokevirtual java_lang_Throwable.fillInStackTraceSignature)::
+      (13%N, Pop)::
+      (14%N, Return)::
+      nil
+    .
+
+    Definition _init_Body : BytecodeMethod := BYTECODEMETHOD.Build_t
+      _init_Instructions
+      nil
+      1
+      2
+    .
+
+    Definition _init_Method : Method := METHOD.Build_t
+      _init_Signature
+      (Some _init_Body)
+      false
+      false
+      false
+      Public
+    .
+
+    Definition class : Class := CLASS.Build_t
+      className
+      (Some java_lang_Object.className)
+      nil
+      nil
+      (_init_Method::nil)
+      false
+      true
+      false
+    .
+
+  End java_lang_Throwable.
